
:Entity a owl:Class ;
     rdfs:label "Entity" ;
     rdfs:comment "Entity is equivalent to the BFO class 'entity' (http://purl.obolibrary.org/obo/BFO_0000001)" .

:Continuant a owl:Class ;
     rdfs:subClassOf :Entity,  [ a owl:Restriction ; owl:onProperty :continuantPartOfAtAllTimes ;  owl:allValuesFrom :Continuant ] ;
     rdfs:label "Continuant" ;
     rdfs:comment "Continuant is equivalent to the BFO class 'continuant' (http://purl.obolibrary.org/obo/BFO_0000002)" .

:Occurrent a owl:Class ;
     rdfs:subClassOf :Entity ;
     rdfs:label "Occurrent" ;
     rdfs:comment "Occurrent is equivalent to the BFO class 'occurrent' (http://purl.obolibrary.org/obo/BFO_0000003)" ;
     owl:disjointWith :Continuant .

:IndependentContinuant a owl:Class ;
     rdfs:subClassOf  [ a owl:Restriction ; owl:onProperty :continuantPartOfAtAllTimes ;  owl:allValuesFrom :IndependentContinuant ], :Continuant ;
     rdfs:label "IndependentContinuant" ;
     rdfs:comment "IndependentContinuant is equivalent to the BFO class 'independent continuant' (http://purl.obolibrary.org/obo/BFO_0000004)" .

:SpatialRegion a owl:Class ;
     rdfs:subClassOf  [ a owl:Restriction ; owl:onProperty :continuantPartOfAtAllTimes ;  owl:allValuesFrom :SpatialRegion ], :ImmaterialEntity ;
     rdfs:label "SpatialRegion" ;
     rdfs:comment "SpatialRegion is equivalent to the BFO class 'spatial region' (http://purl.obolibrary.org/obo/BFO_0000006)" .

:TemporalRegion a owl:Class ;
     rdfs:subClassOf :Occurrent,  [ a owl:Restriction ; owl:onProperty :occurrentPartOf ;  owl:allValuesFrom :TemporalRegion ],  [ a owl:Restriction ; owl:onProperty :temporalPartOf ;  owl:allValuesFrom :TemporalRegion ] ;
     rdfs:label "TemporalRegion" ;
     rdfs:comment "TemporalRegion is equivalent to the BFO class 'temporal region' (http://purl.obolibrary.org/obo/BFO_0000008)" .

:TwoDimensionalSpatialRegion a owl:Class ;
     rdfs:subClassOf :SpatialRegion,  [ a owl:Restriction ; owl:onProperty :hasContinuantPartAtAllTimes ;  owl:allValuesFrom  [ a owl:Class ; owl:unionOf  (:TwoDimensionalSpatialRegion :OneDimensionalSpatialRegion :ZeroDimensionalSpatialRegion) ] ] ;
     rdfs:label "TwoDimensionalSpatialRegion" ;
     rdfs:comment "TwoDimensionalSpatialRegion is equivalent to the BFO class 'two-dimensional spatial region' (http://purl.obolibrary.org/obo/BFO_0000009)" .

:SpatiotemporalRegion a owl:Class ;
     rdfs:subClassOf :Occurrent,  [ a owl:Restriction ; owl:onProperty :occurrentPartOf ;  owl:allValuesFrom :SpatiotemporalRegion ],  [ a owl:Restriction ; owl:onProperty :temporalPartOf ;  owl:allValuesFrom :SpatiotemporalRegion ] ;
     rdfs:label "SpatiotemporalRegion" ;
     rdfs:comment "SpatiotemporalRegion is equivalent to the BFO class 'spatiotemporal region' (http://purl.obolibrary.org/obo/BFO_0000011)" .

:Process a owl:Class ;
     rdfs:subClassOf  [ a owl:Restriction ; owl:onProperty :hasOccurrentPart ;  owl:allValuesFrom  [ a owl:Class ; owl:unionOf  (:Process :ProcessBoundary) ] ],  [ a owl:Restriction ; owl:onProperty :occurrentPartOf ;  owl:allValuesFrom :Process ], :Occurrent ;
     rdfs:label "Process" ;
     rdfs:comment "Process is equivalent to the BFO class 'process' (http://purl.obolibrary.org/obo/BFO_0000015)" .

:Disposition a owl:Class ;
     rdfs:subClassOf :RealizableEntity ;
     rdfs:label "Disposition" ;
     rdfs:comment "Disposition is equivalent to the BFO class 'disposition' (http://purl.obolibrary.org/obo/BFO_0000016)" .

:RealizableEntity a owl:Class ;
     rdfs:subClassOf :SpecificallyDependentContinuant ;
     rdfs:label "RealizableEntity" ;
     rdfs:comment "RealizableEntity is equivalent to the BFO class 'realizable entity' (http://purl.obolibrary.org/obo/BFO_0000017)" ;
     owl:disjointWith :Quality .

:ZeroDimensionalSpatialRegion a owl:Class ;
     rdfs:subClassOf  [ a owl:Restriction ; owl:onProperty :hasContinuantPartAtAllTimes ;  owl:allValuesFrom :ZeroDimensionalSpatialRegion ], :SpatialRegion ;
     rdfs:label "ZeroDimensionalSpatialRegion" ;
     rdfs:comment "ZeroDimensionalSpatialRegion is equivalent to the BFO class 'zero-dimensional spatial region' (http://purl.obolibrary.org/obo/BFO_0000018)" .

:Quality a owl:Class ;
     rdfs:subClassOf :SpecificallyDependentContinuant ;
     rdfs:label "Quality" ;
     rdfs:comment "Quality is equivalent to the BFO class 'quality' (http://purl.obolibrary.org/obo/BFO_0000019)" .

:SpecificallyDependentContinuant a owl:Class ;
     rdfs:subClassOf :Continuant ;
     rdfs:label "SpecificallyDependentContinuant" ;
     rdfs:comment "SpecificallyDependentContinuant is equivalent to the BFO class 'specifically dependent continuant' (http://purl.obolibrary.org/obo/BFO_0000020)" .

:Role a owl:Class ;
     rdfs:subClassOf :RealizableEntity ;
     rdfs:label "Role" ;
     rdfs:comment "Role is equivalent to the BFO class 'role' (http://purl.obolibrary.org/obo/BFO_0000023)" ;
     owl:disjointWith :Disposition .

:FiatObjectPart a owl:Class ;
     rdfs:subClassOf :MaterialEntity ;
     rdfs:label "FiatObjectPart" ;
     rdfs:comment "FiatObjectPart is equivalent to the BFO class 'fiat object part' (http://purl.obolibrary.org/obo/BFO_0000024)" .

:OneDimensionalSpatialRegion a owl:Class ;
     rdfs:subClassOf :SpatialRegion,  [ a owl:Restriction ; owl:onProperty :hasContinuantPartAtAllTimes ;  owl:allValuesFrom  [ a owl:Class ; owl:unionOf  (:OneDimensionalSpatialRegion :ZeroDimensionalSpatialRegion) ] ] ;
     rdfs:label "OneDimensionalSpatialRegion" ;
     rdfs:comment "OneDimensionalSpatialRegion is equivalent to the BFO class 'one-dimensional spatial region' (http://purl.obolibrary.org/obo/BFO_0000026)" .

:ObjectAggregate a owl:Class ;
     rdfs:subClassOf :MaterialEntity ;
     rdfs:label "ObjectAggregate" ;
     rdfs:comment "ObjectAggregate is equivalent to the BFO class 'object aggregate' (http://purl.obolibrary.org/obo/BFO_0000027)" .

:ThreeDimensionalSpatialRegion a owl:Class ;
     rdfs:subClassOf :SpatialRegion,  [ a owl:Restriction ; owl:onProperty :hasContinuantPartAtAllTimes ;  owl:allValuesFrom :SpatialRegion ] ;
     rdfs:label "ThreeDimensionalSpatialRegion" ;
     rdfs:comment "ThreeDimensionalSpatialRegion is equivalent to the BFO class 'three-dimensional spatial region' (http://purl.obolibrary.org/obo/BFO_0000028)" .

:Site a owl:Class ;
     rdfs:subClassOf  [ a owl:Restriction ; owl:onProperty :occupiesSpatialRegionAtAllTimes ;  owl:allValuesFrom :ThreeDimensionalSpatialRegion ], :ImmaterialEntity,  [ a owl:Restriction ; owl:onProperty :hasContinuantPartAtAllTimes ;  owl:allValuesFrom  [ a owl:Class ; owl:unionOf  (:Site :ContinuantFiatBoundary) ] ],  [ a owl:Restriction ; owl:onProperty :continuantPartOfAtAllTimes ;  owl:allValuesFrom  [ a owl:Class ; owl:unionOf  (:Site :MaterialEntity) ] ] ;
     rdfs:label "Site" ;
     rdfs:comment "Site is equivalent to the BFO class 'site' (http://purl.obolibrary.org/obo/BFO_0000029)" .

:Object a owl:Class ;
     rdfs:subClassOf :MaterialEntity ;
     rdfs:label "Object" ;
     rdfs:comment "Object is equivalent to the BFO class 'object' (http://purl.obolibrary.org/obo/BFO_0000030)" .

:GenericallyDependentContinuant a owl:Class ;
     rdfs:subClassOf :Continuant ;
     rdfs:label "GenericallyDependentContinuant" ;
     rdfs:comment "GenericallyDependentContinuant is equivalent to the BFO class 'generically dependent continuant' (http://purl.obolibrary.org/obo/BFO_0000031)" .

:Function a owl:Class ;
     rdfs:subClassOf :Disposition ;
     rdfs:label "Function" ;
     rdfs:comment "Function is equivalent to the BFO class 'function' (http://purl.obolibrary.org/obo/BFO_0000034)" .

:ProcessBoundary a owl:Class ;
     rdfs:subClassOf  [ a owl:Restriction ; owl:onProperty :hasOccurrentPart ;  owl:allValuesFrom :ProcessBoundary ],  [ a owl:Restriction ; owl:onProperty :occurrentPartOf ;  owl:allValuesFrom  [ a owl:Class ; owl:unionOf  (:Process :ProcessBoundary) ] ],  [ a owl:Restriction ; owl:onProperty :hasTemporalPart ;  owl:allValuesFrom :ProcessBoundary ], :Occurrent ;
     rdfs:label "ProcessBoundary" ;
     rdfs:comment "ProcessBoundary is equivalent to the BFO class 'process boundary' (http://purl.obolibrary.org/obo/BFO_0000035)" .

:OneDimensionalTemporalRegion a owl:Class ;
     rdfs:subClassOf  [ a owl:Restriction ; owl:onProperty :temporalPartOf ;  owl:allValuesFrom :OneDimensionalTemporalRegion ], :TemporalRegion,  [ a owl:Restriction ; owl:onProperty :hasTemporalPart ;  owl:allValuesFrom  [ a owl:Class ; owl:unionOf  (:OneDimensionalTemporalRegion :ZeroDimensionalTemporalRegion) ] ] ;
     rdfs:label "OneDimensionalTemporalRegion" ;
     rdfs:comment "OneDimensionalTemporalRegion is equivalent to the BFO class 'one-dimensional temporal region' (http://purl.obolibrary.org/obo/BFO_0000038)" .

:MaterialEntity a owl:Class ;
     rdfs:subClassOf  [ a owl:Restriction ; owl:onProperty :hasContinuantPartAtAllTimes ;  owl:allValuesFrom  [ a owl:Class ; owl:unionOf  (:Site :ContinuantFiatBoundary :MaterialEntity) ] ],  [ a owl:Restriction ; owl:onProperty :continuantPartOfAtAllTimes ;  owl:allValuesFrom :MaterialEntity ], :IndependentContinuant ;
     rdfs:label "MaterialEntity" ;
     rdfs:comment "MaterialEntity is equivalent to the BFO class 'material entity' (http://purl.obolibrary.org/obo/BFO_0000040)" .

:ContinuantFiatBoundary a owl:Class ;
     rdfs:subClassOf  [ a owl:Restriction ; owl:onProperty :locationOfAtAllTimes ;  owl:allValuesFrom :ContinuantFiatBoundary ],  [ a owl:Restriction ; owl:onProperty :hasContinuantPartAtAllTimes ;  owl:allValuesFrom :ContinuantFiatBoundary ], :ImmaterialEntity ;
     rdfs:label "ContinuantFiatBoundary" ;
     rdfs:comment "ContinuantFiatBoundary is equivalent to the BFO class 'continuant fiat boundary' (http://purl.obolibrary.org/obo/BFO_0000140)" .

:ImmaterialEntity a owl:Class ;
     rdfs:subClassOf :IndependentContinuant ;
     rdfs:label "ImmaterialEntity" ;
     rdfs:comment "ImmaterialEntity is equivalent to the BFO class 'immaterial entity' (http://purl.obolibrary.org/obo/BFO_0000141)" ;
     owl:disjointWith :MaterialEntity .

:FiatLine a owl:Class ;
     rdfs:subClassOf  [ a owl:Restriction ; owl:onProperty :hasContinuantPartAtAllTimes ;  owl:allValuesFrom  [ a owl:Class ; owl:unionOf  (:FiatLine :FiatPoint) ] ], :ContinuantFiatBoundary ;
     rdfs:label "FiatLine" ;
     rdfs:comment "FiatLine is equivalent to the BFO class 'fiat line' (http://purl.obolibrary.org/obo/BFO_0000142)" .

:RelationalQuality a owl:Class ;
     rdfs:subClassOf :Quality ;
     rdfs:label "RelationalQuality" ;
     rdfs:comment "RelationalQuality is equivalent to the BFO class 'relational quality' (http://purl.obolibrary.org/obo/BFO_0000145)" .

:FiatSurface a owl:Class ;
     rdfs:subClassOf  [ a owl:Restriction ; owl:onProperty :hasContinuantPartAtAllTimes ;  owl:allValuesFrom :ContinuantFiatBoundary ], :ContinuantFiatBoundary ;
     rdfs:label "FiatSurface" ;
     rdfs:comment "FiatSurface is equivalent to the BFO class 'fiat surface' (http://purl.obolibrary.org/obo/BFO_0000146)" .

:FiatPoint a owl:Class ;
     rdfs:subClassOf :ContinuantFiatBoundary,  [ a owl:Restriction ; owl:onProperty :hasContinuantPartAtAllTimes ;  owl:allValuesFrom :FiatPoint ] ;
     rdfs:label "FiatPoint" ;
     rdfs:comment "FiatPoint is equivalent to the BFO class 'fiat point' (http://purl.obolibrary.org/obo/BFO_0000147)" .

:ZeroDimensionalTemporalRegion a owl:Class ;
     rdfs:subClassOf :TemporalRegion,  [ a owl:Restriction ; owl:onProperty :hasTemporalPart ;  owl:allValuesFrom :ZeroDimensionalTemporalRegion ] ;
     rdfs:label "ZeroDimensionalTemporalRegion" ;
     rdfs:comment "ZeroDimensionalTemporalRegion is equivalent to the BFO class 'zero-dimensional temporal region' (http://purl.obolibrary.org/obo/BFO_0000148)" ;
     owl:disjointWith :OneDimensionalTemporalRegion .

:History a owl:Class ;
     rdfs:subClassOf :Process ;
     rdfs:label "History" ;
     rdfs:comment "History is equivalent to the BFO class 'history' (http://purl.obolibrary.org/obo/BFO_0000182)" .

:TimeInterval a owl:Class ;
     rdfs:subClassOf :OneDimensionalTemporalRegion ;
     rdfs:label "TimeInterval" ;
     rdfs:comment "TimeInterval is equivalent to the BFO class 'temporal interval' (http://purl.obolibrary.org/obo/BFO_0000202)" .

:TimeInstant a owl:Class ;
     rdfs:subClassOf :ZeroDimensionalTemporalRegion ;
     rdfs:label "TimeInstant" ;
     rdfs:comment "TimeInstant is equivalent to the BFO class 'temporal instant' (http://purl.obolibrary.org/obo/BFO_0000203)" .
 
:hasRealization a owl:ObjectProperty ;
     rdfs:label "hasRealization" ;
     rdfs:comment "hasRealization is equivalent to the BFO property 'has realization' (http://purl.obolibrary.org/obo/BFO_0000054)" ;
     rdfs:domain :RealizableEntity ;
     rdfs:range :Process .
 
:realizes a owl:ObjectProperty ;
     rdfs:label "realizes" ;
     rdfs:comment "realizes is equivalent to the BFO property 'realizes' (http://purl.obolibrary.org/obo/BFO_0000055)" ;
     rdfs:domain :Process ;
     rdfs:range :RealizableEntity .
 
:participatesIn a owl:ObjectProperty ;
     rdfs:label "participatesIn" ;
     rdfs:comment "participatesIn is equivalent to the BFO property 'participates in at some time' (http://purl.obolibrary.org/obo/BFO_0000056)" ;
     rdfs:domain  [ a owl:Class ; owl:unionOf  ( [ a owl:Class ; owl:intersectionOf  (:IndependentContinuant  [ a owl:Class ; owl:complementOf :SpatialRegion ]) ] :SpecificallyDependentContinuant :GenericallyDependentContinuant) ] ;
     rdfs:range :Process .
 
:hasParticipant a owl:ObjectProperty ;
     rdfs:label "hasParticipant" ;
     rdfs:comment "hasParticipant is equivalent to the BFO property 'has participant at some time' (http://purl.obolibrary.org/obo/BFO_0000057)" ;
     rdfs:domain :Process ;
     rdfs:range  [ a owl:Class ; owl:unionOf  ( [ a owl:Class ; owl:intersectionOf  (:IndependentContinuant  [ a owl:Class ; owl:complementOf :SpatialRegion ]) ] :SpecificallyDependentContinuant :GenericallyDependentContinuant) ] .
 
:isConcretizedBy a owl:ObjectProperty ;
     rdfs:label "isConcretizedBy" ;
     rdfs:comment "isConcretizedBy is equivalent to the BFO property 'is concretized by at some time' (http://purl.obolibrary.org/obo/BFO_0000058)" ;
     rdfs:domain :GenericallyDependentContinuant ;
     rdfs:range  [ a owl:Class ; owl:unionOf  (:SpecificallyDependentContinuant :Process) ] .
 
:concretizes a owl:ObjectProperty ;
     rdfs:label "concretizes" ;
     rdfs:comment "concretizes is equivalent to the BFO property 'concretizes at some time' (http://purl.obolibrary.org/obo/BFO_0000059)" ;
     rdfs:domain  [ a owl:Class ; owl:unionOf  (:SpecificallyDependentContinuant :Process) ] ;
     rdfs:range :GenericallyDependentContinuant .
 
:precededBy a owl:ObjectProperty, owl:TransitiveProperty ;
     rdfs:label "precededBy" ;
     rdfs:comment "precededBy is equivalent to the BFO property 'preceded by' (http://purl.obolibrary.org/obo/BFO_0000062)" ;
     rdfs:domain :Occurrent ;
     rdfs:range :Occurrent .
 
:precedes a owl:ObjectProperty, owl:TransitiveProperty ;
     rdfs:label "precedes" ;
     rdfs:comment "precedes is equivalent to the BFO property 'precedes' (http://purl.obolibrary.org/obo/BFO_0000063)" ;
     rdfs:domain :Occurrent ;
     rdfs:range :Occurrent .
 
:occursIn a owl:ObjectProperty ;
     rdfs:label "occursIn" ;
     rdfs:comment "occursIn is equivalent to the BFO property 'occurs in' (http://purl.obolibrary.org/obo/BFO_0000066)" ;
     rdfs:domain  [ a owl:Class ; owl:unionOf  (:Process :ProcessBoundary) ] ;
     rdfs:range  [ a owl:Class ; owl:unionOf  (:MaterialEntity :Site) ] .
 
:locatedInAtAllTimes a owl:ObjectProperty, owl:TransitiveProperty ;
     rdfs:subPropertyOf :locatedIn ;
     rdfs:label "locatedInAtAllTimes" ;
     rdfs:comment "locatedInAtAllTimes is equivalent to the BFO property 'located in at all times' (http://purl.obolibrary.org/obo/BFO_0000082)" ;
     rdfs:domain  [ a owl:Class ; owl:intersectionOf  (:IndependentContinuant  [ a owl:Class ; owl:complementOf :SpatialRegion ]) ] ;
     rdfs:range  [ a owl:Class ; owl:intersectionOf  (:IndependentContinuant  [ a owl:Class ; owl:complementOf :SpatialRegion ]) ] .
 
:genericallyDependsOn a owl:ObjectProperty ;
     rdfs:label "genericallyDependsOn" ;
     rdfs:comment "genericallyDependsOn is equivalent to the BFO property 'generically depends on at some time' (http://purl.obolibrary.org/obo/BFO_0000084)" ;
     rdfs:domain :GenericallyDependentContinuant ;
     rdfs:range  [ a owl:Class ; owl:intersectionOf  (:IndependentContinuant  [ a owl:Class ; owl:complementOf :SpatialRegion ]) ] .
 
:isCarrierOf a owl:ObjectProperty ;
     rdfs:label "isCarrierOf" ;
     rdfs:comment "isCarrierOf is equivalent to the BFO property 'is carrier of at some time' (http://purl.obolibrary.org/obo/BFO_0000101)" ;
     rdfs:domain  [ a owl:Class ; owl:intersectionOf  (:IndependentContinuant  [ a owl:Class ; owl:complementOf :SpatialRegion ]) ] ;
     rdfs:range :GenericallyDependentContinuant .
 
:existsAt a owl:ObjectProperty ;
     rdfs:label "existsAt" ;
     rdfs:comment "existsAt is equivalent to the BFO property 'exists at' (http://purl.obolibrary.org/obo/BFO_0000108)" .
 
:hasContinuantPartAtAllTimes a owl:ObjectProperty, owl:TransitiveProperty ;
     rdfs:subPropertyOf :hasContinuantPart ;
     rdfs:label "hasContinuantPartAtAllTimes" ;
     rdfs:comment "hasContinuantPartAtAllTimes is equivalent to the BFO property 'has continuant part at all times' (http://purl.obolibrary.org/obo/BFO_0000110)" ;
     rdfs:domain :Continuant ;
     rdfs:range :Continuant .
 
:hasProperContinuantPartAtAllTimes a owl:TransitiveProperty, owl:ObjectProperty ;
     rdfs:subPropertyOf :hasProperContinuantPart, :hasContinuantPartAtAllTimes ;
     rdfs:label "hasProperContinuantPartAtAllTimes" ;
     rdfs:comment "hasProperContinuantPartAtAllTimes is equivalent to the BFO property 'has proper continuant part at all times' (http://purl.obolibrary.org/obo/BFO_0000111)" ;
     rdfs:domain :Continuant ;
     rdfs:range :Continuant .
 
:hasMaterialBasisAtAllTimes a owl:ObjectProperty ;
     rdfs:subPropertyOf :hasMaterialBasis ;
     rdfs:label "hasMaterialBasisAtAllTimes" ;
     rdfs:comment "hasMaterialBasisAtAllTimes is equivalent to the BFO property 'has material basis at all times' (http://purl.obolibrary.org/obo/BFO_0000113)" ;
     rdfs:domain :Disposition ;
     rdfs:range :MaterialEntity .
 
:hasMemberPart a owl:ObjectProperty ;
     rdfs:subPropertyOf :hasContinuantPart ;
     rdfs:label "hasMemberPart" ;
     rdfs:comment "hasMemberPart is equivalent to the BFO property 'has member part at some time' (http://purl.obolibrary.org/obo/BFO_0000115)" ;
     rdfs:domain :MaterialEntity ;
     rdfs:range :MaterialEntity .
 
:hasOccurrentPart a owl:TransitiveProperty, owl:ObjectProperty ;
     rdfs:subPropertyOf :hasPart ;
     rdfs:label "hasOccurrentPart" ;
     rdfs:comment "hasOccurrentPart is equivalent to the BFO property 'has occurrent part' (http://purl.obolibrary.org/obo/BFO_0000117)" ;
     rdfs:domain :Occurrent ;
     rdfs:range :Occurrent .
 
:hasProperOccurrentPart a owl:ObjectProperty ;
     rdfs:subPropertyOf :hasOccurrentPart ;
     rdfs:label "hasProperOccurrentPart" ;
     rdfs:comment "hasProperOccurrentPart is equivalent to the BFO property 'has proper occurrent part' (http://purl.obolibrary.org/obo/BFO_0000118)" ;
     rdfs:domain :Occurrent ;
     rdfs:range :Occurrent .
 
:hasTemporalPart a owl:ObjectProperty, owl:TransitiveProperty ;
     rdfs:subPropertyOf :hasOccurrentPart ;
     rdfs:label "hasTemporalPart" ;
     rdfs:comment "hasTemporalPart is equivalent to the BFO property 'has temporal part' (http://purl.obolibrary.org/obo/BFO_0000121)" ;
     rdfs:domain :Occurrent ;
     rdfs:range :Occurrent .
 
:locationOf a owl:ObjectProperty ;
     rdfs:label "locationOf" ;
     rdfs:comment "locationOf is equivalent to the BFO property 'location of at some time' (http://purl.obolibrary.org/obo/BFO_0000124)" ;
     rdfs:domain  [ a owl:Class ; owl:intersectionOf  (:IndependentContinuant  [ a owl:Class ; owl:complementOf :SpatialRegion ]) ] ;
     rdfs:range  [ a owl:Class ; owl:intersectionOf  (:IndependentContinuant  [ a owl:Class ; owl:complementOf :SpatialRegion ]) ] .
 
:materialBasisOf a owl:ObjectProperty ;
     rdfs:label "materialBasisOf" ;
     rdfs:comment "materialBasisOf is equivalent to the BFO property 'material basis of at some time' (http://purl.obolibrary.org/obo/BFO_0000127)" ;
     rdfs:domain :MaterialEntity ;
     rdfs:range :Disposition .
 
:memberPartOf a owl:ObjectProperty ;
     rdfs:subPropertyOf :continuantPartOf ;
     rdfs:label "memberPartOf" ;
     rdfs:comment "memberPartOf is equivalent to the BFO property 'member part of at some time' (http://purl.obolibrary.org/obo/BFO_0000129)" ;
     rdfs:domain :MaterialEntity ;
     rdfs:range :MaterialEntity .
 
:occurrentPartOf a owl:ObjectProperty, owl:TransitiveProperty ;
     rdfs:subPropertyOf :isPartOf ;
     rdfs:label "occurrentPartOf" ;
     rdfs:comment "occurrentPartOf is equivalent to the BFO property 'occurrent part of' (http://purl.obolibrary.org/obo/BFO_0000132)" ;
     rdfs:domain :Occurrent ;
     rdfs:range :Occurrent .
 
:properTemporalPartOf a owl:ObjectProperty ;
     rdfs:subPropertyOf :temporalPartOf ;
     rdfs:label "properTemporalPartOf" ;
     rdfs:comment "properTemporalPartOf is equivalent to the BFO property 'proper temporal part of' (http://purl.obolibrary.org/obo/BFO_0000136)" ;
     rdfs:domain :Occurrent ;
     rdfs:range :Occurrent .
 
:properContinuantPartOfAtAllTimes a owl:ObjectProperty, owl:TransitiveProperty ;
     rdfs:subPropertyOf :continuantPartOfAtAllTimes, :properContinuantPartOf ;
     rdfs:label "properContinuantPartOfAtAllTimes" ;
     rdfs:comment "properContinuantPartOfAtAllTimes is equivalent to the BFO property 'proper continuant part of at all times' (http://purl.obolibrary.org/obo/BFO_0000137)" ;
     rdfs:domain :Continuant ;
     rdfs:range :Continuant .
 
:properOccurrentPartOf a owl:ObjectProperty ;
     rdfs:subPropertyOf :occurrentPartOf ;
     rdfs:label "properOccurrentPartOf" ;
     rdfs:comment "properOccurrentPartOf is equivalent to the BFO property 'proper occurrent part of' (http://purl.obolibrary.org/obo/BFO_0000138)" ;
     rdfs:domain :Occurrent ;
     rdfs:range :Occurrent .
 
:temporalPartOf a owl:ObjectProperty, owl:TransitiveProperty ;
     rdfs:subPropertyOf :occurrentPartOf ;
     rdfs:label "temporalPartOf" ;
     rdfs:comment "temporalPartOf is equivalent to the BFO property 'temporal part of' (http://purl.obolibrary.org/obo/BFO_0000139)" ;
     rdfs:domain :Occurrent ;
     rdfs:range :Occurrent .
 
:temporallyProjectsOnto a owl:FunctionalProperty, owl:ObjectProperty ;
     rdfs:label "temporallyProjectsOnto" ;
     rdfs:comment "temporallyProjectsOnto is equivalent to the BFO property 'temporally projects onto' (http://purl.obolibrary.org/obo/BFO_0000153)" ;
     rdfs:domain :SpatiotemporalRegion ;
     rdfs:range :TemporalRegion .
 
:materialBasisOfAtAllTimes a owl:ObjectProperty ;
     rdfs:subPropertyOf :materialBasisOf ;
     rdfs:label "materialBasisOfAtAllTimes" ;
     rdfs:comment "materialBasisOfAtAllTimes is equivalent to the BFO property 'material basis of at all times' (http://purl.obolibrary.org/obo/BFO_0000163)" ;
     rdfs:domain :MaterialEntity ;
     rdfs:range :Disposition .
 
:concretizesAtAllTimes a owl:ObjectProperty ;
     rdfs:subPropertyOf :concretizes ;
     rdfs:label "concretizesAtAllTimes" ;
     rdfs:comment "concretizesAtAllTimes is equivalent to the BFO property 'concretizes at all times' (http://purl.obolibrary.org/obo/BFO_0000164)" ;
     rdfs:domain  [ a owl:Class ; owl:unionOf  (:SpecificallyDependentContinuant :Process) ] ;
     rdfs:range :GenericallyDependentContinuant .
 
:isConcretizedByAtAllTimes a owl:ObjectProperty ;
     rdfs:subPropertyOf :isConcretizedBy ;
     rdfs:label "isConcretizedByAtAllTimes" ;
     rdfs:comment "isConcretizedByAtAllTimes is equivalent to the BFO property 'is concretized by at all times' (http://purl.obolibrary.org/obo/BFO_0000165)" ;
     rdfs:domain :GenericallyDependentContinuant ;
     rdfs:range  [ a owl:Class ; owl:unionOf  (:SpecificallyDependentContinuant :Process) ] .
 
:participatesInAtAllTimes a owl:ObjectProperty ;
     rdfs:subPropertyOf :participatesIn ;
     rdfs:label "participatesInAtAllTimes" ;
     rdfs:comment "participatesInAtAllTimes is equivalent to the BFO property 'participates in at all times' (http://purl.obolibrary.org/obo/BFO_0000166)" ;
     rdfs:domain  [ a owl:Class ; owl:unionOf  ( [ a owl:Class ; owl:intersectionOf  (:IndependentContinuant  [ a owl:Class ; owl:complementOf :SpatialRegion ]) ] :SpecificallyDependentContinuant :GenericallyDependentContinuant) ] ;
     rdfs:range :Process .
 
:hasParticipantAtAllTimes a owl:ObjectProperty ;
     rdfs:subPropertyOf :hasParticipant ;
     rdfs:label "hasParticipantAtAllTimes" ;
     rdfs:comment "hasParticipantAtAllTimes is equivalent to the BFO property 'has participant at all times' (http://purl.obolibrary.org/obo/BFO_0000167)" ;
     rdfs:domain :Process ;
     rdfs:range  [ a owl:Class ; owl:unionOf  ( [ a owl:Class ; owl:intersectionOf  (:IndependentContinuant  [ a owl:Class ; owl:complementOf :SpatialRegion ]) ] :SpecificallyDependentContinuant :GenericallyDependentContinuant) ] .
 
:locationOfAtAllTimes a owl:ObjectProperty, owl:TransitiveProperty ;
     rdfs:subPropertyOf :locationOf ;
     rdfs:label "locationOfAtAllTimes" ;
     rdfs:comment "locationOfAtAllTimes is equivalent to the BFO property 'location of at all times' (http://purl.obolibrary.org/obo/BFO_0000170)" ;
     rdfs:domain  [ a owl:Class ; owl:intersectionOf  (:IndependentContinuant  [ a owl:Class ; owl:complementOf :SpatialRegion ]) ] ;
     rdfs:range  [ a owl:Class ; owl:intersectionOf  (:IndependentContinuant  [ a owl:Class ; owl:complementOf :SpatialRegion ]) ] .
 
:locatedIn a owl:ObjectProperty ;
     rdfs:label "locatedIn" ;
     rdfs:comment "locatedIn is equivalent to the BFO property 'located in at some time' (http://purl.obolibrary.org/obo/BFO_0000171)" ;
     rdfs:domain  [ a owl:Class ; owl:intersectionOf  (:IndependentContinuant  [ a owl:Class ; owl:complementOf :SpatialRegion ]) ] ;
     rdfs:range  [ a owl:Class ; owl:intersectionOf  (:IndependentContinuant  [ a owl:Class ; owl:complementOf :SpatialRegion ]) ] .
 
:hasMemberPartAtAllTimes a owl:ObjectProperty ;
     rdfs:subPropertyOf :hasMemberPart, :hasContinuantPartAtAllTimes ;
     rdfs:label "hasMemberPartAtAllTimes" ;
     rdfs:comment "hasMemberPartAtAllTimes is equivalent to the BFO property 'has member part at all times' (http://purl.obolibrary.org/obo/BFO_0000172)" ;
     rdfs:domain :MaterialEntity ;
     rdfs:range :MaterialEntity .
 
:memberPartOfAtAllTimes a owl:ObjectProperty ;
     rdfs:subPropertyOf :continuantPartOfAtAllTimes, :memberPartOf ;
     rdfs:label "memberPartOfAtAllTimes" ;
     rdfs:comment "memberPartOfAtAllTimes is equivalent to the BFO property 'member part of at all times' (http://purl.obolibrary.org/obo/BFO_0000173)" ;
     rdfs:domain :MaterialEntity ;
     rdfs:range :MaterialEntity .
 
:hasProperContinuantPart a owl:ObjectProperty ;
     rdfs:subPropertyOf :hasContinuantPart ;
     rdfs:label "hasProperContinuantPart" ;
     rdfs:comment "hasProperContinuantPart is equivalent to the BFO property 'has proper continuant part at some time' (http://purl.obolibrary.org/obo/BFO_0000174)" ;
     rdfs:domain :Continuant ;
     rdfs:range :Continuant .
 
:properContinuantPartOf a owl:ObjectProperty ;
     rdfs:subPropertyOf :continuantPartOf ;
     rdfs:label "properContinuantPartOf" ;
     rdfs:comment "properContinuantPartOf is equivalent to the BFO property 'proper continuant part of at some time' (http://purl.obolibrary.org/obo/BFO_0000175)" ;
     rdfs:domain :Continuant ;
     rdfs:range :Continuant .
 
:continuantPartOf a owl:ObjectProperty ;
     rdfs:subPropertyOf :isPartOf ;
     rdfs:label "continuantPartOf" ;
     rdfs:comment "continuantPartOf is equivalent to the BFO property 'continuant part of at some time' (http://purl.obolibrary.org/obo/BFO_0000176)" ;
     rdfs:domain :Continuant ;
     rdfs:range :Continuant .
 
:continuantPartOfAtAllTimes a owl:ObjectProperty, owl:TransitiveProperty ;
     rdfs:subPropertyOf :continuantPartOf ;
     rdfs:label "continuantPartOfAtAllTimes" ;
     rdfs:comment "continuantPartOfAtAllTimes is equivalent to the BFO property 'continuant part of at all times' (http://purl.obolibrary.org/obo/BFO_0000177)" ;
     rdfs:domain :Continuant ;
     rdfs:range :Continuant .
 
:hasContinuantPart a owl:ObjectProperty ;
     rdfs:subPropertyOf :hasPart ;
     rdfs:label "hasContinuantPart" ;
     rdfs:comment "hasContinuantPart is equivalent to the BFO property 'has continuant part at some time' (http://purl.obolibrary.org/obo/BFO_0000178)" ;
     rdfs:domain :Continuant ;
     rdfs:range :Continuant .
 
:hasProperTemporalPart a owl:ObjectProperty ;
     rdfs:subPropertyOf :hasTemporalPart ;
     rdfs:label "hasProperTemporalPart" ;
     rdfs:comment "hasProperTemporalPart is equivalent to the BFO property 'has proper temporal part' (http://purl.obolibrary.org/obo/BFO_0000181)" ;
     rdfs:domain :Occurrent ;
     rdfs:range :Occurrent .
 
:environs a owl:ObjectProperty ;
     rdfs:label "environs" ;
     rdfs:comment "environs is equivalent to the BFO property 'environs' (http://purl.obolibrary.org/obo/BFO_0000183)" ;
     rdfs:domain  [ a owl:Class ; owl:unionOf  (:MaterialEntity :Site) ] ;
     rdfs:range  [ a owl:Class ; owl:unionOf  (:Process :ProcessBoundary) ] .
 
:historyOf a owl:InverseFunctionalProperty, owl:FunctionalProperty, owl:ObjectProperty ;
     rdfs:label "historyOf" ;
     rdfs:comment "historyOf is equivalent to the BFO property 'history of' (http://purl.obolibrary.org/obo/BFO_0000184)" ;
     rdfs:domain :History ;
     rdfs:range :MaterialEntity .
 
:hasHistory a owl:ObjectProperty ;
     rdfs:label "hasHistory" ;
     rdfs:comment "hasHistory is equivalent to the BFO property 'has history' (http://purl.obolibrary.org/obo/BFO_0000185)" ;
     rdfs:domain :MaterialEntity ;
     rdfs:range :History .
 
:specificallyDependedOnBy a owl:ObjectProperty ;
     rdfs:label "specificallyDependedOnBy" ;
     rdfs:comment "specificallyDependedOnBy is equivalent to the BFO property 'specifically depended on by' (http://purl.obolibrary.org/obo/BFO_0000194)" ;
     rdfs:domain  [ a owl:Class ; owl:unionOf  (:SpecificallyDependentContinuant  [ a owl:Class ; owl:intersectionOf  (:IndependentContinuant  [ a owl:Class ; owl:complementOf :SpatialRegion ]) ]) ] ;
     rdfs:range :SpecificallyDependentContinuant .
 
:specificallyDependsOn a owl:ObjectProperty ;
     rdfs:label "specificallyDependsOn" ;
     rdfs:comment "specificallyDependsOn is equivalent to the BFO property 'specifically depends on' (http://purl.obolibrary.org/obo/BFO_0000195)" ;
     rdfs:domain :SpecificallyDependentContinuant ;
     rdfs:range  [ a owl:Class ; owl:unionOf  (:SpecificallyDependentContinuant  [ a owl:Class ; owl:intersectionOf  (:IndependentContinuant  [ a owl:Class ; owl:complementOf :SpatialRegion ]) ]) ] .
 
:bearerOf a owl:ObjectProperty ;
     rdfs:subPropertyOf :specificallyDependedOnBy ;
     rdfs:label "bearerOf" ;
     rdfs:comment "bearerOf is equivalent to the BFO property 'bearer of' (http://purl.obolibrary.org/obo/BFO_0000196)" ;
     rdfs:domain  [ a owl:Class ; owl:intersectionOf  (:IndependentContinuant  [ a owl:Class ; owl:complementOf :SpatialRegion ]) ] ;
     rdfs:range :SpecificallyDependentContinuant .
 
:inheresIn a owl:ObjectProperty ;
     rdfs:subPropertyOf :specificallyDependsOn ;
     rdfs:label "inheresIn" ;
     rdfs:comment "inheresIn is equivalent to the BFO property 'inheres in' (http://purl.obolibrary.org/obo/BFO_0000197)" ;
     rdfs:domain :SpecificallyDependentContinuant ;
     rdfs:range  [ a owl:Class ; owl:intersectionOf  (:IndependentContinuant  [ a owl:Class ; owl:complementOf :SpatialRegion ]) ] .
 
:occupiesTemporalRegion a owl:FunctionalProperty, owl:ObjectProperty ;
     rdfs:label "occupiesTemporalRegion" ;
     rdfs:comment "occupiesTemporalRegion is equivalent to the BFO property 'occupies temporal region' (http://purl.obolibrary.org/obo/BFO_0000199)" ;
     rdfs:domain  [ a owl:Class ; owl:unionOf  (:Process :ProcessBoundary) ] ;
     rdfs:range :TemporalRegion .
 
:occupiesSpatiotemporalRegion a owl:ObjectProperty, owl:FunctionalProperty ;
     rdfs:label "occupiesSpatiotemporalRegion" ;
     rdfs:comment "occupiesSpatiotemporalRegion is equivalent to the BFO property 'occupies spatiotemporal region' (http://purl.obolibrary.org/obo/BFO_0000200)" ;
     rdfs:domain  [ a owl:Class ; owl:unionOf  (:Process :ProcessBoundary) ] ;
     rdfs:range :SpatiotemporalRegion .
 
:occupiesSpatialRegion a owl:ObjectProperty ;
     rdfs:label "occupiesSpatialRegion" ;
     rdfs:comment "occupiesSpatialRegion is equivalent to the BFO property 'occupies spatial region at some time' (http://purl.obolibrary.org/obo/BFO_0000210)" ;
     rdfs:domain  [ a owl:Class ; owl:intersectionOf  (:IndependentContinuant  [ a owl:Class ; owl:complementOf :SpatialRegion ]) ] ;
     rdfs:range :SpatialRegion .
 
:occupiesSpatialRegionAtAllTimes a owl:ObjectProperty, owl:FunctionalProperty ;
     rdfs:subPropertyOf :occupiesSpatialRegion ;
     rdfs:label "occupiesSpatialRegionAtAllTimes" ;
     rdfs:comment "occupiesSpatialRegionAtAllTimes is equivalent to the BFO property 'occupies spatial region at all times' (http://purl.obolibrary.org/obo/BFO_0000211)" ;
     rdfs:domain  [ a owl:Class ; owl:intersectionOf  (:IndependentContinuant  [ a owl:Class ; owl:complementOf :SpatialRegion ]) ] ;
     rdfs:range :SpatialRegion .
 
:spatiallyProjectsOnto a owl:ObjectProperty ;
     rdfs:label "spatiallyProjectsOnto" ;
     rdfs:comment "spatiallyProjectsOnto is equivalent to the BFO property 'spatially projects onto at some time' (http://purl.obolibrary.org/obo/BFO_0000216)" ;
     rdfs:domain :SpatiotemporalRegion ;
     rdfs:range :SpatialRegion .
 
:spatiallyProjectsOntoAtAllTimes a owl:FunctionalProperty, owl:ObjectProperty ;
     rdfs:subPropertyOf :spatiallyProjectsOnto ;
     rdfs:label "spatiallyProjectsOntoAtAllTimes" ;
     rdfs:comment "spatiallyProjectsOntoAtAllTimes is equivalent to the BFO property 'spatially projects onto at all times' (http://purl.obolibrary.org/obo/BFO_0000217)" ;
     rdfs:domain :SpatiotemporalRegion ;
     rdfs:range :SpatialRegion .
 
:hasMaterialBasis a owl:ObjectProperty ;
     rdfs:label "hasMaterialBasis" ;
     rdfs:comment "hasMaterialBasis is equivalent to the BFO property 'has material basis at some time' (http://purl.obolibrary.org/obo/BFO_0000218)" ;
     rdfs:domain :Disposition ;
     rdfs:range :MaterialEntity .
 
:genericallyDependsOnAtAllTimes a owl:ObjectProperty ;
     rdfs:subPropertyOf :genericallyDependsOn ;
     rdfs:label "genericallyDependsOnAtAllTimes" ;
     rdfs:comment "genericallyDependsOnAtAllTimes is equivalent to the BFO property 'generically depends on at all times' (http://purl.obolibrary.org/obo/BFO_0000219)" ;
     rdfs:domain :GenericallyDependentContinuant ;
     rdfs:range  [ a owl:Class ; owl:intersectionOf  (:IndependentContinuant  [ a owl:Class ; owl:complementOf :SpatialRegion ]) ] .
 
:isCarrierOfAtAllTimes a owl:ObjectProperty ;
     rdfs:subPropertyOf :isCarrierOf ;
     rdfs:label "isCarrierOfAtAllTimes" ;
     rdfs:comment "isCarrierOfAtAllTimes is equivalent to the BFO property 'is carrier of at all times' (http://purl.obolibrary.org/obo/BFO_0000220)" ;
     rdfs:domain  [ a owl:Class ; owl:intersectionOf  (:IndependentContinuant  [ a owl:Class ; owl:complementOf :SpatialRegion ]) ] ;
     rdfs:range :GenericallyDependentContinuant .
 
:firstInstantOf a owl:ObjectProperty ;
     rdfs:label "firstInstantOf" ;
     rdfs:comment "firstInstantOf is equivalent to the BFO property 'first instant of' (http://purl.obolibrary.org/obo/BFO_0000221)" ;
     rdfs:domain :TimeInstant ;
     rdfs:range :TemporalRegion .
 
:hasFirstInstant a owl:FunctionalProperty, owl:ObjectProperty ;
     rdfs:label "hasFirstInstant" ;
     rdfs:comment "hasFirstInstant is equivalent to the BFO property 'has first instant' (http://purl.obolibrary.org/obo/BFO_0000222)" ;
     rdfs:domain :TemporalRegion ;
     rdfs:range :TimeInstant .
 
:lastInstantOf a owl:ObjectProperty ;
     rdfs:label "lastInstantOf" ;
     rdfs:comment "lastInstantOf is equivalent to the BFO property 'last instant of' (http://purl.obolibrary.org/obo/BFO_0000223)" ;
     rdfs:domain :TimeInstant ;
     rdfs:range :TemporalRegion .
 
:hasLastInstant a owl:ObjectProperty, owl:FunctionalProperty ;
     rdfs:label "hasLastInstant" ;
     rdfs:comment "hasLastInstant is equivalent to the BFO property 'has last instant' (http://purl.obolibrary.org/obo/BFO_0000224)" ;
     rdfs:domain :TemporalRegion ;
     rdfs:range :TimeInstant .
